coq/proof/SoundPostcondCmd.v
@@ -25,6 +25,9 @@ Require InvState.
 Require Import Inject.
 Require Import SoundBase.
 Require Import SoundForget.
+Require Import SoundPostcondCmdCheck.
+Require Import SoundPostcondCmdForget.
+Require Import SoundPostcondCmdAdd.
 
 Set Implicit Arguments.
 
@@ -40,130 +43,6 @@ Proof.
   destruct c_src, c_tgt; ss; des_ifs.
 Qed.
 
-(* TODO: we can assume source's progress *)
-Lemma postcond_cmd_check_sound
-      conf_src st0_src cmd_src cmds_src def_src uses_src
-      conf_tgt st0_tgt cmd_tgt cmds_tgt def_tgt uses_tgt
-      invst0 invmem0 inv0
-      st1_tgt evt
-      (POSTCOND: Postcond.postcond_cmd_check cmd_src cmd_tgt def_src def_tgt uses_src uses_tgt inv0)
-      (STATE: InvState.Rel.sem conf_src conf_tgt st0_src st0_tgt invst0 invmem0 inv0)
-      (MEM: InvMem.Rel.sem conf_src conf_tgt st0_src.(Mem) st0_tgt.(Mem) invmem0)
-      (STEP_TGT: sInsn conf_tgt st0_tgt st1_tgt evt)
-      (CMDS_SRC: st0_src.(EC).(CurCmds) = cmd_src :: cmds_src)
-      (CMDS_TGT: st0_tgt.(EC).(CurCmds) = cmd_tgt :: cmds_tgt)
-      (NONCALL_SRC: ~ Instruction.isCallInst cmd_src)
-      (NONCALL_TGT: ~ Instruction.isCallInst cmd_tgt)
-      (DEF_SRC: def_src = AtomSetImpl_from_list (option_to_list (Cmd.get_def cmd_src)))
-      (DEF_TGT: def_tgt = AtomSetImpl_from_list (option_to_list (Cmd.get_def cmd_tgt)))
-      (USES_SRC: uses_src = AtomSetImpl_from_list (Cmd.get_ids cmd_src))
-      (USES_TGT: uses_tgt = AtomSetImpl_from_list (Cmd.get_ids cmd_tgt)):
-  exists st1_src,
-    <<STEP_SRC: sInsn conf_src st0_src st1_src evt>>.
-Proof.
-Admitted.
-
-Definition FORGET_MEMORY_TODO: Prop. Admitted. (* TODO *)
-
-(* TODO: we can assume source's progress *)
-Lemma postcond_cmd_forget_sound
-      conf_src st0_src st1_src def_src leaks_src cmd_src cmds_src
-      conf_tgt st0_tgt st1_tgt def_tgt leaks_tgt cmd_tgt cmds_tgt
-      invst0 invmem0 inv0
-      (STATE: InvState.Rel.sem conf_src conf_tgt st0_src st0_tgt invst0 invmem0 inv0)
-      (MEM: InvMem.Rel.sem conf_src conf_tgt st0_src.(Mem) st0_tgt.(Mem) invmem0)
-      (CMDS_SRC: st0_src.(EC).(CurCmds) = cmd_src :: cmds_src)
-      (CMDS_TGT: st0_tgt.(EC).(CurCmds) = cmd_tgt :: cmds_tgt)
-      (STATE_SRC: state_equiv_except def_src st0_src st1_src)
-      (STATE_TGT: state_equiv_except def_tgt st0_tgt st1_tgt)
-      (UNIQUE_SRC: unique_preserved_except conf_src invst0.(InvState.Rel.src) inv0.(Invariant.src) st1_src def_src leaks_src)
-      (UNIQUE_TGT: unique_preserved_except conf_tgt invst0.(InvState.Rel.tgt) inv0.(Invariant.tgt) st1_tgt def_tgt leaks_tgt)
-      (MEM_SRC: FORGET_MEMORY_TODO)
-      (MEM_TGT: FORGET_MEMORY_TODO)
-  : exists invst1 invmem1,
-    <<STATE: InvState.Rel.sem conf_src conf_tgt st1_src st1_tgt invst1 invmem1
-                              (Postcond.postcond_cmd_forget
-                                 cmd_src cmd_tgt
-                                 def_src def_tgt leaks_src leaks_tgt
-                                 inv0)>> /\
-    <<MEM: InvMem.Rel.sem conf_src conf_tgt st1_src.(Mem) st1_tgt.(Mem) invmem1>> /\
-    <<MEMLE: InvMem.Rel.le invmem0 invmem1>>.
-Proof.
-Admitted.
-
-Lemma postcond_cmd_add_sound
-      conf_src st0_src st1_src cmd_src cmds_src def_src uses_src
-      conf_tgt st0_tgt st1_tgt cmd_tgt cmds_tgt def_tgt uses_tgt
-      invst0 invmem0 inv0
-      evt
-      (POSTCOND: Postcond.postcond_cmd_check cmd_src cmd_tgt def_src def_tgt uses_src uses_tgt inv0)
-      (STATE: InvState.Rel.sem conf_src conf_tgt st1_src st1_tgt invst0 invmem0 inv0)
-      (MEM: InvMem.Rel.sem conf_src conf_tgt st1_src.(Mem) st1_tgt.(Mem) invmem0)
-      (STEP_SRC: sInsn conf_src st0_src st1_src evt)
-      (STEP_TGT: sInsn conf_tgt st0_tgt st1_tgt evt)
-      (CMDS_SRC: st0_src.(EC).(CurCmds) = cmd_src :: cmds_src)
-      (CMDS_TGT: st0_tgt.(EC).(CurCmds) = cmd_tgt :: cmds_tgt)
-      (NONCALL_SRC: ~ Instruction.isCallInst cmd_src)
-      (NONCALL_TGT: ~ Instruction.isCallInst cmd_tgt)
-      (DEF_SRC: def_src = AtomSetImpl_from_list (option_to_list (Cmd.get_def cmd_src)))
-      (DEF_TGT: def_tgt = AtomSetImpl_from_list (option_to_list (Cmd.get_def cmd_tgt)))
-      (USES_SRC: uses_src = AtomSetImpl_from_list (Cmd.get_ids cmd_src))
-      (USES_TGT: uses_tgt = AtomSetImpl_from_list (Cmd.get_ids cmd_tgt)):
-  exists invst1 invmem1,
-    <<STATE: InvState.Rel.sem conf_src conf_tgt st1_src st1_tgt invst1 invmem1
-                              (Postcond.postcond_cmd_add cmd_src cmd_tgt inv0)>> /\
-    <<MEM: InvMem.Rel.sem conf_src conf_tgt st1_src.(Mem) st1_tgt.(Mem) invmem1>> /\
-    <<MEMLE: InvMem.Rel.le invmem0 invmem1>>.
-Proof.
-Admitted.
-
-Definition Invariant_le (inv0 inv1: Invariant.t): Prop. Admitted. (* TODO *)
-
-Lemma postcond_cmd_check_mon
-          src tgt
-          def_src def_tgt uses_src uses_tgt
-          inv0 inv1
-          (LE: Invariant_le inv0 inv1)
-          (CHECK: postcond_cmd_check
-                    src tgt
-                    def_src def_tgt uses_src uses_tgt
-                    inv0):
-  postcond_cmd_check
-    src tgt
-    def_src def_tgt uses_src uses_tgt
-    inv1.
-Proof.
-Admitted.
-
-Lemma postcond_cmd_forget_le
-      def_src def_tgt leaks_src leaks_tgt
-      def_memory_src def_memory_tgt
-      inv:
-  Invariant_le
-    (postcond_cmd_forget
-       def_src def_tgt leaks_src leaks_tgt
-       def_memory_src def_memory_tgt
-       inv)
-    inv.
-Proof.
-Admitted.
-
-Lemma step_state_equiv_except
-      cmd cmds
-      conf st0 st1 evt
-      (CMDS: st0.(EC).(CurCmds) = cmd :: cmds)
-      (STEP: sInsn conf st0 st1 evt)
-  : state_equiv_except (AtomSetImpl_from_list (option_to_list (Cmd.get_def cmd))) st0 st1.
-Proof.
-Admitted.
-
-(* TODO: complete this lemma about unique_preserved_except *)
-(* Lemma step_unique_preserved_except *)
-(*           (STEP: sInsn conf_src st0_src st1_src evt) *)
-(*     : unique_preserved_except conf_src (InvState.Rel.src invst0) (Invariant.src inv0) *)
-(*     (AtomSetImpl_from_list (Cmd.get_def ?Goal13)) ?Goal *)
-
-(* TODO: we can assume source's progress *)
 Lemma postcond_cmd_sound
       conf_src st0_src cmd_src cmds_src
       conf_tgt st0_tgt cmd_tgt cmds_tgt
@@ -176,7 +55,8 @@ Lemma postcond_cmd_sound
       (CMDS_SRC: st0_src.(EC).(CurCmds) = cmd_src :: cmds_src)
       (CMDS_TGT: st0_tgt.(EC).(CurCmds) = cmd_tgt :: cmds_tgt)
       (NONCALL_SRC: ~ Instruction.isCallInst cmd_src)
-      (NONCALL_TGT: ~ Instruction.isCallInst cmd_tgt):
+      (NONCALL_TGT: ~ Instruction.isCallInst cmd_tgt)
+      (NERROR_SRC: ~ error_state conf_src st0_src):
   exists st1_src invst1 invmem1,
     <<STEP_SRC: sInsn conf_src st0_src st1_src evt>> /\
     <<STATE: InvState.Rel.sem conf_src conf_tgt st1_src st1_tgt invst1 invmem1 inv1>> /\
