coq/proof/SimulationValid.v
@@ -267,7 +267,7 @@ Proof.
       esplits; (try by etransitivity; eauto); eauto.
       { econs 1. eauto. }
       instantiate (1 := mkState (mkEC _ _ _ _ _ _) _ _).
-      right. apply CIH. econs; try exact STATE3; eauto.
+      right. apply CIH. econs; try exact x1; eauto.
 Admitted.
 
 Lemma valid_sim_fdef
