coq/proof/SoundPostcondCmdCheck.v
@@ -1,0 +1,104 @@
+Require Import syntax.
+Require Import alist.
+Require Import FMapWeakList.
+
+Require Import Classical.
+Require Import Coqlib.
+Require Import infrastructure.
+Require Import Metatheory.
+Import LLVMsyntax.
+Import LLVMinfra.
+Require Import opsem.
+
+Require Import sflib.
+Require Import paco.
+Import Opsem.
+
+Require Import TODO.
+Require Import Exprs.
+Require Import Hints.
+Require Import Postcond.
+Require Import Validator.
+Require Import GenericValues.
+Require InvMem.
+Require InvState.
+Require Import Inject.
+Require Import SoundBase.
+Require Import SoundForget.
+
+Set Implicit Arguments.
+
+
+Definition Invariant_le (inv0 inv1: Invariant.t): Prop. Admitted. (* TODO *)
+
+Lemma postcond_cmd_check_mon
+          src tgt
+          def_src def_tgt uses_src uses_tgt
+          inv0 inv1
+          (LE: Invariant_le inv0 inv1)
+          (CHECK: postcond_cmd_check
+                    src tgt
+                    def_src def_tgt uses_src uses_tgt
+                    inv0):
+  postcond_cmd_check
+    src tgt
+    def_src def_tgt uses_src uses_tgt
+    inv1.
+Proof.
+Admitted.
+
+Lemma postcond_cmd_forget_le
+      def_src def_tgt leaks_src leaks_tgt
+      def_memory_src def_memory_tgt
+      inv:
+  Invariant_le
+    (postcond_cmd_forget
+       def_src def_tgt leaks_src leaks_tgt
+       def_memory_src def_memory_tgt
+       inv)
+    inv.
+Proof.
+Admitted.
+
+
+Lemma event_call
+      conf st0 st1 evt cmd cmds
+      (STEP: sInsn conf st0 st1 evt)
+      (CMDS: st0.(EC).(CurCmds) = cmd::cmds)
+      (NONCALL: ~ Instruction.isCallInst cmd):
+  evt = events.E0.
+Proof.
+  inv STEP; ss. inv CMDS. ss. congruence.
+Qed.
+
+Lemma postcond_cmd_check_sound
+      conf_src st0_src cmd_src cmds_src def_src uses_src
+      conf_tgt st0_tgt cmd_tgt cmds_tgt def_tgt uses_tgt
+      invst0 invmem0 inv0
+      st1_tgt evt
+      (POSTCOND: Postcond.postcond_cmd_check cmd_src cmd_tgt def_src def_tgt uses_src uses_tgt inv0)
+      (STATE: InvState.Rel.sem conf_src conf_tgt st0_src st0_tgt invst0 invmem0 inv0)
+      (MEM: InvMem.Rel.sem conf_src conf_tgt st0_src.(Mem) st0_tgt.(Mem) invmem0)
+      (STEP_TGT: sInsn conf_tgt st0_tgt st1_tgt evt)
+      (CMDS_SRC: st0_src.(EC).(CurCmds) = cmd_src :: cmds_src)
+      (CMDS_TGT: st0_tgt.(EC).(CurCmds) = cmd_tgt :: cmds_tgt)
+      (NONCALL_SRC: ~ Instruction.isCallInst cmd_src)
+      (NONCALL_TGT: ~ Instruction.isCallInst cmd_tgt)
+      (NERROR_SRC: ~ error_state conf_src st0_src)
+      (DEF_SRC: def_src = AtomSetImpl_from_list (option_to_list (Cmd.get_def cmd_src)))
+      (DEF_TGT: def_tgt = AtomSetImpl_from_list (option_to_list (Cmd.get_def cmd_tgt)))
+      (USES_SRC: uses_src = AtomSetImpl_from_list (Cmd.get_ids cmd_src))
+      (USES_TGT: uses_tgt = AtomSetImpl_from_list (Cmd.get_ids cmd_tgt)):
+  exists st1_src,
+    <<STEP_SRC: sInsn conf_src st0_src st1_src evt>>.
+Proof.
+  destruct (s_isFinialState conf_src st0_src) eqn:FINAL.
+  { unfold s_isFinialState in FINAL. simtac. }
+  exploit nerror_nfinal_nstuck; eauto. i. des.
+  replace e with evt in *.
+  { esplits; eauto. }
+  unfold postcond_cmd_check in POSTCOND. simtac.
+  exploit (@event_call conf_src); eauto. i.
+  exploit (@event_call conf_tgt); eauto. i.
+  subst. ss.
+Qed.
