coq/proof/SoundPostcondCmdForget.v
@@ -1,0 +1,74 @@
+Require Import syntax.
+Require Import alist.
+Require Import FMapWeakList.
+
+Require Import Classical.
+Require Import Coqlib.
+Require Import infrastructure.
+Require Import Metatheory.
+Import LLVMsyntax.
+Import LLVMinfra.
+Require Import opsem.
+
+Require Import sflib.
+Require Import paco.
+Import Opsem.
+
+Require Import TODO.
+Require Import Exprs.
+Require Import Hints.
+Require Import Postcond.
+Require Import Validator.
+Require Import GenericValues.
+Require InvMem.
+Require InvState.
+Require Import Inject.
+Require Import SoundBase.
+Require Import SoundForget.
+
+Set Implicit Arguments.
+
+
+Lemma step_state_equiv_except
+      cmd cmds
+      conf st0 st1 evt
+      (CMDS: st0.(EC).(CurCmds) = cmd :: cmds)
+      (STEP: sInsn conf st0 st1 evt)
+  : state_equiv_except (AtomSetImpl_from_list (option_to_list (Cmd.get_def cmd))) st0 st1.
+Proof.
+Admitted.
+
+(* TODO: complete this lemma about unique_preserved_except *)
+(* Lemma step_unique_preserved_except *)
+(*           (STEP: sInsn conf_src st0_src st1_src evt) *)
+(*     : unique_preserved_except conf_src (InvState.Rel.src invst0) (Invariant.src inv0) *)
+(*     (AtomSetImpl_from_list (Cmd.get_def ?Goal13)) ?Goal *)
+
+
+Definition FORGET_MEMORY_TODO: Prop. Admitted. (* TODO *)
+
+(* TODO: we can assume source's progress *)
+Lemma postcond_cmd_forget_sound
+      conf_src st0_src st1_src def_src leaks_src cmd_src cmds_src
+      conf_tgt st0_tgt st1_tgt def_tgt leaks_tgt cmd_tgt cmds_tgt
+      invst0 invmem0 inv0
+      (STATE: InvState.Rel.sem conf_src conf_tgt st0_src st0_tgt invst0 invmem0 inv0)
+      (MEM: InvMem.Rel.sem conf_src conf_tgt st0_src.(Mem) st0_tgt.(Mem) invmem0)
+      (CMDS_SRC: st0_src.(EC).(CurCmds) = cmd_src :: cmds_src)
+      (CMDS_TGT: st0_tgt.(EC).(CurCmds) = cmd_tgt :: cmds_tgt)
+      (STATE_SRC: state_equiv_except def_src st0_src st1_src)
+      (STATE_TGT: state_equiv_except def_tgt st0_tgt st1_tgt)
+      (UNIQUE_SRC: unique_preserved_except conf_src invst0.(InvState.Rel.src) inv0.(Invariant.src) st1_src def_src leaks_src)
+      (UNIQUE_TGT: unique_preserved_except conf_tgt invst0.(InvState.Rel.tgt) inv0.(Invariant.tgt) st1_tgt def_tgt leaks_tgt)
+      (MEM_SRC: FORGET_MEMORY_TODO)
+      (MEM_TGT: FORGET_MEMORY_TODO)
+  : exists invst1 invmem1,
+    <<STATE: InvState.Rel.sem conf_src conf_tgt st1_src st1_tgt invst1 invmem1
+                              (Postcond.postcond_cmd_forget
+                                 cmd_src cmd_tgt
+                                 def_src def_tgt leaks_src leaks_tgt
+                                 inv0)>> /\
+    <<MEM: InvMem.Rel.sem conf_src conf_tgt st1_src.(Mem) st1_tgt.(Mem) invmem1>> /\
+    <<MEMLE: InvMem.Rel.le invmem0 invmem1>>.
+Proof.
+Admitted.
